\documentclass[9pt]{extarticle}

\usepackage[hmargin=0.5in,tmargin=0.5in]{geometry}
\usepackage{amsmath,amssymb}
\usepackage{times}
\usepackage{graphicx}
\usepackage{subfigure}

\usepackage{cleveref}
\usepackage{color}
\newcommand{\TODO}[1]{\textcolor{red}{#1}}

\newcommand{\FPP}[2]{\frac{\partial #1}{\partial #2}}
\newcommand{\argmin}{\operatornamewithlimits{arg\ min}}
\author{Siwang Li}

\title{implicit integration}

%% document begin here
\begin{document}
\maketitle

\setlength{\parskip}{0.5ex}

\section{Integration}
\begin{equation}
  M\ddot{u} + (\alpha_mM + \alpha_kK)\dot{u}+f(u) = f_{ext}
\end{equation}

\begin{equation}
  M \frac{u_{k+1}-2u_k+u_{k-1}}{h^2} + (\alpha_mM + \alpha_kK)\frac{u_{k+1}-u_{k}}{h}+f(u_{k}+hv_{k+1}) = f_{ext}
\end{equation}

\begin{equation}
  v_{k+1} = \frac{u_{k+1}-u_{k}}{h}
\end{equation}

\begin{equation}
  f(u_{k}+hv_{k+1}) = f(u_k) + hKv_{k+1} = f(u_k)+K({u_{k+1}-u_{k}})
\end{equation}

\begin{equation} 
  (\frac{1}{h^2}M + \frac{(\alpha_mM + \alpha_kK)}{h}+K)u_{k+1} = f_{ext}-(M\frac{-2u_k+u_{k-1}}{h^2}-\frac{(\alpha_mM + \alpha_kK)}{h}u_k+f(u_k)-Ku_k)
\end{equation}

\begin{equation}
  A = (\frac{1}{h^2}M + \frac{(\alpha_mM + \alpha_kK)}{h}+K)
\end{equation}

\begin{equation} 
  b = f_{ext}-(M\frac{-2u_k+u_{k-1}}{h^2}-\frac{(\alpha_mM + \alpha_kK)}{h}u_k+f(u_k)-Ku_k)
\end{equation}

\begin{equation}
  A (x_{k+1}-x_0) = b
\end{equation}

\begin{equation}
  A x_{k+1} = b+Ax_0
\end{equation}

\begin{equation}
  u_{k+1} = x_{k+1}-x_0
\end{equation}

\begin{equation}
  v_{k+1} = \frac{u_{k+1}-u_{k}}{h}
\end{equation}

\end{document}